fowl/Provides/OptionTheorems.v
@@ -4,6 +4,13 @@ From Maniunfold Require Export
 Definition is_Some (A : Type) (x : option A) : bool :=
   if x then true else false.
 
+Definition option_bind (A B : Type)
+  (f : A -> option B) (x : option A) : option B :=
+  match x with
+  | Some a => f a
+  | None => None
+  end.
+
 Lemma option_map_id (A : Type) (x : option A) :
   option_map id x = x.
 Proof. destruct x as [a |]; auto. Qed.
